nonchalant work

src/multiplier.v
@@ -1,502 +1,268 @@
-(**********************************************************************************)
-(*                                                                                *)
-(*             multiplier.v - Shift-and-add 4-bit multiplier.                     *)
-(*                                                                                *)
-(*                   +---------------------------+                                *)
-(*                   |                           |                                *)
-(*           A -----------                 ------|------ P                        *)
-(*                   |                           |                                *)
-(*           B -----------        A*B            |                                *)
-(*                   |                           |                                *)
-(*           V -----------                 ------------- R                        *)
-(*                   |                           |                                *)
-(*                   +---------------------------+                                *)
-(*                                                                                *)
-(*  The main theorem is a statement of a cryptographic constant-time (CCT)        *)
-(*  hyperproperty. The statement of the property looks as follows (which we       *)
-(*  state as an equivalent single-copy trace property):                           *)
-(*                                                                                *)
-(*  There exists some predictor [f] such that given a circuit_step schedule [C],  *)
-(*  starting from a reset state, the multiplier circuit [M] will produce an       *)
-(*  implementation leakage trace [t'].                                            *)
-(*                                                                                *)
-(*  A specification leakage trace [t] is extracted from schedule [C] which        *)
-(*  will record the values of [A] and [valid] each circuit_step. On termination,  *)
-(*                                                                                *)
-(*                              [t' = f t].                                       *)
-(*                                                                                *)
-(**********************************************************************************)
+From research Require Import base bit program simulates.
 
-From research Require Import base bitvector.
+Notation Maybe := @option.
 
-Local Open Scope bv_scope.
+Inductive spec := | Spec__Enq (a : Bit 4) | Spec__Deq | Spec__Tick.
+Inductive impl := | Impl__Enq | Impl__Deq | Impl__Tick.
+Inductive method := | Method__Enq (a b : Bit 4) | Method__Deq | Method__Tick.
+Inductive state := State__Empty | State__Busy | State__Full.
+Instance state__EqDecision : EqDecision state. solve_decision. Defined.
 
-Section definitions.
-  Record Registers :=
-    { r_A : bv 8
-    ; r_B : bv 4
-    ; r_cnt : bv 2
-    ; r_busy : bv 1
+Definition policy m :=
+  match m with
+  | Method__Enq a b => Spec__Enq a
+  | Method__Deq => Spec__Deq
+  | Method__Tick => Spec__Tick
+  end.
+
+Module Impl.
+  Record t_inner :=
+    { a : Bit 4
+    ; b : Bit 4
+    ; c : Bit 2
+    ; p : Bit 8
+    ; st : state
+    ; trace : list impl
     }.
 
-  Record I :=
-    { in_A : bv 4
-    ; in_B : bv 4
-    ; in_valid : bv 1
-    }.
+  Definition t := t_inner.
 
-  Record O :=
-    { out_P : bv 8
-    ; out_ready : bv 1
-    }.
+  Definition mk : t :=
+    {| a := 0%bv
+    ; b := 0%bv
+    ; c := 0%bv
+    ; p := 0%bv
+    ; st := State__Empty
+    ; trace := []
+    |}.
 
-  Definition O0 := {| out_P := 0; out_ready := 0 |}.
+  Definition enq in1 in2 :=
+    {{ st' <- $st ;;
+       when (decide (st' = State__Empty)) then
+         trace ↩ Impl__Enq ;;
+         a <=: in1 ;;
+         b <=: in2 ;;
+         c <=: 0%bv ;;
+         p <=: 0%bv ;;
+         st <=: State__Busy
+    }}.
 
-  Record ILeakage :=
-    { leak_valid : bv 1
-    ; leak_ready : bv 1
-    }.
+  Definition deq :=
+    {{ st' <- $st ;;
+       if (decide (st' = State__Full)) then
+         trace ↩ Impl__Deq ;;
+         st <=: State__Empty ;;
+         p' <- $p ;;
+         ret (Valid p')
+       else
+         ret Invalid
+    }}.
 
-  Record State :=
-    { R : Registers
-    ; T : list ILeakage
-    ; Y : list O
-    }.
+  Definition shift_and_add :=
+    {{ a' <- $a ;;
+       b' <- $b ;;
+       c' <- $c ;;
+       p' <- $p ;;
+       when decide (a' <> 0%bv) then
+         let t :=
+           if decide ((truncate a' : Bit 1) = 1)%bv then
+             (zeroExtend b' : Bit 8)%bv
+           else
+             0%bv
+         in
+         p <=: (p' + (t ≪ (zeroExtend c' : Bit 8)))%bv ;;
+         a <=: (a' ≫ 1)%bv ;;
+         c <=: (c' + 1)%bv
+    }}.
 
-  Definition State0 :=
-    {| R := {| r_A := 0; r_B := 0; r_cnt := 0; r_busy := 0 |}
-    ; T := []
-    ; Y := [] |}.
+  Definition tick :=
+    {{ st' <- $st ;;
+       when (decide (st' = State__Busy)) then
+         trace ↩ Impl__Tick ;;
+         a' <- $a ;;
+         if (decide (a' = 0%bv)) then
+           st <=: State__Full
+         else
+           shift_and_add
+    }}.
 
-  Definition shift_and_add (b : bv 4) (a : bv 8) : bv 8 :=
-    let t0 := bv_extract 4 5 a in
-    let t1 := if a? then 5#b else 0 in
-    t0 + t1 || bv_extract 1 3 a.
-
-  Definition circuit_step (s : State) (x : I) : State :=
-    if s.(R).(r_busy) =? 0
-    then
-      if x.(in_valid) =? 1
-      then
-        let ra' := 8#x.(in_A) in
-        let rb' := x.(in_B) in
-        let rcount' := 3 in
-        let rbusy' := 1 in
-        let r' := {| r_A := ra'; r_B := rb'; r_cnt := rcount'; r_busy := rbusy' |} in
-        let t' := s.(T) ++ [{| leak_valid := 1; leak_ready := 0 |}] in
-        let y' := s.(Y) ++ [O0] in
-        {| R := r'; T := t'; Y := y' |}
-      else
-        let t' := s.(T) ++ [{| leak_valid := 0; leak_ready := 0 |}] in
-        let r' := s.(R) in
-        let y' := s.(Y) ++ [O0] in
-        {| R := r'; T := t'; Y := y' |}
-    else
-      let ra' := shift_and_add s.(R).(r_B) s.(R).(r_A) in
-      let rb' := s.(R).(r_B) in
-      if s.(R).(r_cnt) =? 0
-      then
-        let rcount' := 0 in
-        let rbusy' := 0 in
-        let r' := {| r_A := ra'; r_B := rb'; r_cnt := rcount'; r_busy := rbusy' |} in
-        let t' := s.(T) ++ [{| leak_valid := x.(in_valid); leak_ready := 1 |}] in
-        let y' := s.(Y) ++ [{| out_P := ra'; out_ready := 1 |}] in
-        {| R := r'; T := t'; Y := y' |}
-      else
-        let rcount' := bv_pred s.(R).(r_cnt) in
-        let rbusy' := 1 in
-        let r' := {| r_A := ra'; r_B := rb'; r_cnt := rcount'; r_busy := rbusy' |} in
-        let t' := s.(T) ++ [{| leak_valid := x.(in_valid); leak_ready := 0 |}] in
-        let y' := s.(Y) ++ [O0] in
-        {| R := r'; T := t'; Y := y' |}.
-
-  Definition circuit_steps s xs := fold_left circuit_step xs s.
-End definitions.
-
-Section correctness.
-  Fixpoint repeat {A : Type} (f : A -> A) (n : nat) {struct n} : (A -> A) :=
-    match n with
-    | 0%nat => id
-    | S n' => f ∘ repeat f n'
+  Definition methodResult m :=
+    match m with
+    | Method__Enq _ _ => unit
+    | Method__Deq => Maybe (Bit 8)
+    | Method__Tick => unit
     end.
 
-  Definition repeat_shift_and_add n b a := (repeat (shift_and_add b) n) a.
-
-  Definition shift_and_add4 := repeat_shift_and_add 4.
-
-  Definition shift_and_add' (b a : Z) :=
-    Z.lor (bv_wrap 5 (a ≫ 4 + (bv_wrap 1 a * b)) ≪ 3) (bv_wrap 3 (a ≫ 1)).
-
-  Definition repeat_shift_and_add' n b a := (repeat (shift_and_add' b) n) a.
-
-  Definition shift_and_add4' := repeat_shift_and_add' 4.
-
-  Lemma shift_and_add_equiv : forall a b,
-      shift_and_add' (bv_unsigned b) (bv_unsigned a) =
-        bv_unsigned (shift_and_add b a).
-  Proof.
-    intros a b. unfold shift_and_add, shift_and_add'. bv_simplify.
-    unfold Z.of_N, bv_odd.
-    unfold bv_wrap. rewrite Zmod_odd. case_match.
-    - replace (1 * bv_unsigned b)%Z with (bv_unsigned b) by lia. bv_solve.
-    - Search (0 * _)%Z. rewrite Z.mul_0_l. bv_solve.
-  Qed.
-
-  Lemma shift_and_add_repeat_equiv : forall n a b,
-      (repeat_shift_and_add' n) (bv_unsigned b) (bv_unsigned a) =
-        bv_unsigned (repeat_shift_and_add n b a).
-  Proof.
-    intros n a b. induction n; simplify.
-    - unfold repeat_shift_and_add', repeat_shift_and_add. equality.
-    - unfold repeat_shift_and_add', repeat_shift_and_add in *. simplify.
-      rewrite IHn. apply shift_and_add_equiv.
-  Qed.
-
-  Lemma shift_and_add4_equiv : forall a b,
-      shift_and_add4' (bv_unsigned b) (bv_unsigned a) =
-        bv_unsigned (shift_and_add4 b a).
-  Proof.
-    unfold shift_and_add4', shift_and_add4. apply shift_and_add_repeat_equiv.
-  Qed.
-
-  (* Tactic for exhaustive case analysis on integers in range [0,16) *)
-  (* Automatically finds variables with range hypotheses and does case analysis *)
-  Ltac by_cases16 :=
-    repeat match goal with
-      | [ H : (0 <= ?z < 16)%Z |- _ ] =>
-          let Hz := fresh "Hcases" in
-          assert (z = 0 \/ z = 1 \/ z = 2 \/ z = 3 \/ z = 4 \/ z = 5 \/ z = 6 \/ z = 7 \/
-                    z = 8 \/ z = 9 \/ z = 10 \/ z = 11 \/ z = 12 \/ z = 13 \/ z = 14 \/ z = 15)%Z
-            as Hz by lia; clear H;
-          destruct_or?; subst
-      end; equality.
-
-  Lemma shift_and_add4'_multiplies : forall a b,
-      (0 <= a < bv_modulus 4%N)%Z ->
-      (0 <= b < bv_modulus 4%N)%Z ->
-      shift_and_add4' b a = (a * b)%Z.
-  Proof.
-    intros a b Ha Hb.
-    replace (bv_modulus 4%N) with 16%Z in * by reflexivity.
-    by_cases16.
-  Qed.
-
-  Lemma shift_and_add4_multiplies : forall (a b : bv 4),
-      bv_unsigned (shift_and_add4 b (8#a)) = (bv_unsigned a * bv_unsigned b)%Z.
-  Proof.
-    intros a b. rewrite <- shift_and_add4_equiv.
-    Search bv_unsigned bv_zero_extend. rewrite bv_zero_extend_unsigned by lia.
-    apply shift_and_add4'_multiplies. all: bv_solve.
-  Qed.
-
-  Notation "a *| b" := ((8#a) * (8#b)) (at level 35).
-
-  Lemma shift_and_add4_correct : forall (a b : bv 4),
-      shift_and_add4 b (8#a) = a *| b.
-  Proof.
-    intros a b. Search (bv_unsigned _ = bv_unsigned _).
-    rewrite bv_eq. Search bv_mul.
-    rewrite bv_mul_unsigned.
-    Search bv_zero_extend bv_unsigned.
-    repeat rewrite bv_zero_extend_unsigned by lia.
-    Check bv_wrap_small. rewrite bv_wrap_small.
-    - apply shift_and_add4_multiplies.
-    - bv_saturate_unsigned. unfold bv_modulus in *; simplify. nia.
-  Qed.
-
-  Definition busy (s : State) := s.(R).(r_busy) = 1.
-  Definition finished (s : State) := s.(R).(r_cnt) = 0.
-  Definition valid (x : I) := x.(in_valid) = 1.
-
-  Definition circuit_step_idle_valid s1 x s2 : Prop :=
-    ~ busy s1 -> valid x -> s2 = circuit_step s1 x ->
-    s2 = s1 <| R := {| r_A := 8#x.(in_A); r_B := x.(in_B); r_cnt := 3; r_busy := 1 |} |>
-            <| T := s1.(T) ++ [{| leak_valid := 1; leak_ready := 0 |}] |>
-            <| Y := s1.(Y) ++ [O0] |>.
-
-  Lemma circuit_step_idle_valid_holds : forall s1 x s2, circuit_step_idle_valid s1 x s2.
-  Proof.
-    unfold circuit_step_idle_valid. simplify.
-    unfold circuit_step in *. unfold busy in *.
-    unfold valid in *. rewrite <- bv_eqb_neq in H.
-    simplify!. rewrite H0. rewrite H.
-    simplify. equality.
-  Qed.
-
-  Definition circuit_step_idle_invalid s1 x s2 : Prop :=
-    ~ busy s1 -> ~ valid x -> s2 = circuit_step s1 x ->
-    s2 = s1 <| T := s1.(T) ++ [{| leak_valid := 0; leak_ready := 0 |}] |>
-            <| Y := s1.(Y) ++ [O0] |>.
-
-  Lemma circuit_step_idle_invalid_holds : forall s1 x s2, circuit_step_idle_invalid s1 x s2.
-  Proof.
-    unfold circuit_step_idle_invalid. simplify.
-    unfold circuit_step, busy, valid in *.
-    simplify!. rewrite H. rewrite H0.
-    simplify. equality.
-  Qed.
-
-  Definition circuit_step_busy_unfinished s1 x s2 : Prop :=
-    busy s1 -> ~ finished s1 -> s2 = circuit_step s1 x ->
-    s2 = s1 <| R; r_A := shift_and_add s1.(R).(r_B) s1.(R).(r_A) |>
-            <| R; r_cnt := bv_pred s1.(R).(r_cnt)|>
-            <| T := s1.(T) ++ [{| leak_valid := x.(in_valid); leak_ready := 0 |}] |>
-            <| Y := s1.(Y) ++ [O0] |> .
-
-  Lemma circuit_step_busy_unfinished_holds : forall s1 x s2, circuit_step_busy_unfinished s1 x s2.
-  Proof.
-    unfold circuit_step_busy_unfinished. simplify.
-    unfold circuit_step, busy, finished in *.
-    simplify!. rewrite H.
-    simplify. rewrite <- bv_eqb_neq in H0. rewrite H0.
-    equality.
-  Qed.
-
-  Definition circuit_step_busy_finished s1 x s2 : Prop :=
-    busy s1 -> finished s1 -> s2 = circuit_step s1 x ->
-    s2 = s1 <| R; r_A := shift_and_add s1.(R).(r_B) s1.(R).(r_A) |>
-            <| R; r_cnt := 0 |>
-            <| R; r_busy := 0 |>
-            <| T := s1.(T) ++ [{| leak_valid := x.(in_valid); leak_ready := 1 |}] |>
-            <| Y := s1.(Y) ++ [{|
-                             out_P := shift_and_add s1.(R).(r_B) s1.(R).(r_A);
-                             out_ready := 1
-                           |}]
-              |>.
-
-  Lemma circuit_step_busy_finished_holds : forall s1 x s2, circuit_step_busy_finished s1 x s2.
-  Proof.
-    unfold circuit_step_busy_finished. simplify.
-    unfold circuit_step, busy, finished in *.
-    rewrite H0. simplify!. rewrite H.
-    simplify. equality.
-  Qed.
-
-  Tactic Notation "unfold*" :=
-    unfold circuit_step_idle_valid, circuit_step_idle_invalid, circuit_step_busy_unfinished,
-      circuit_step_busy_finished, circuit_steps, busy, finished, shift_and_add4,
-      valid, repeat_shift_and_add, repeat, compose in *.
-
-  (* Finally, with all those helper theorems out of the way, we can now prove
-     the following correctness property:
-
-     For any circuit_step where the circuit is idle, if a valid [a] and [b] are
-     provided, four circuit_steps later it will produce [a *| b]. *)
-
-  Theorem circuit_steps_correct: forall s1 x1 s2 x2 s3 x3 s4 x4 s5 x5 s6 a b,
-      ~ busy s1 ->
-      x1 = {| in_A := a; in_B := b; in_valid := 1 |} ->
-      s2 = circuit_step s1 x1 ->
-      s3 = circuit_step s2 x2 ->
-      s4 = circuit_step s3 x3 ->
-      s5 = circuit_step s4 x4 ->
-      s6 = circuit_step s5 x5 ->
-      s6.(Y) = s1.(Y) ++ [O0; O0; O0; O0; {| out_P := a *| b; out_ready := 1 |}].
-  Proof.
-    intros. rewrite <- shift_and_add4_correct. unfold*. simpl in *.
-
-    1: apply circuit_step_idle_valid_holds      in H1.
-    1: apply circuit_step_busy_unfinished_holds in H2.
-    1: apply circuit_step_busy_unfinished_holds in H3.
-    1: apply circuit_step_busy_unfinished_holds in H4.
-    1: apply circuit_step_busy_finished_holds   in H5.
-
-    all: unfold*; simplify; solve [ eauto | bv_solve ].
-  Qed.
-End correctness.
-
-Section ct.
-  Definition SLeakage := option unit.
-
-  Definition public1 x := if x.(in_valid) =? 1 then Some tt else None.
-
-  Definition public := map public1.
-
-  Definition PredictorState := option nat.
-
-  Definition predictor_step (st : PredictorState) (s : SLeakage) :=
-    match st with
-    | Some (S n) => Some n
-    | Some 0%nat => None
-    | None =>
-        match s with
-        | Some _ => Some 3%nat
-        | None   => None
-        end
+  Definition runMethod m : ActionValue (methodResult m) :=
+    match m with
+    | Method__Enq a b => enq a b
+    | Method__Deq => deq
+    | Method__Tick => tick
     end.
 
-  Definition predictor_steps (st : PredictorState) (xs : list SLeakage) :=
-    fold_left predictor_step xs st.
+  Definition runMethod1 m := runAction1 (runMethod m).
+  Definition runMethods xs := fold_left (fun a b => runMethod1 b a) xs.
 
-  Definition predict_next (st : PredictorState) (s : SLeakage) :=
-    match st with
-    | Some 0%nat =>
-        match s with
-        | Some _ => {| leak_valid := 1; leak_ready := 1 |}
-        | None => {| leak_valid := 0; leak_ready := 1 |}
-        end
-    | _ =>
-        match s with
-        | Some _ => {| leak_valid := 1; leak_ready := 0 |}
-        | None => {| leak_valid := 0; leak_ready := 0 |}
-        end
+  Definition circuit : Circuit t method := {| init := mk; run := runMethod1 |}.
+End Impl.
+
+Module Spec.
+  Record t_inner :=
+    { st : state
+    ; a : Bit 4
+    ; trace : list impl
+    }.
+
+  Definition t := t_inner.
+
+  Definition mk : t :=
+    {| st := State__Empty
+    ; a := 0%bv
+    ; trace := []
+    |}.
+
+  Definition enq in1 :=
+    {{ st' <- $st ;;
+       when (decide (st' = State__Empty)) then
+         trace ↩ Impl__Enq ;;
+         a <=: in1 ;;
+         st <=: State__Busy
+    }}.
+
+  Definition deq :=
+    {{ st' <- $st ;;
+       when (decide (st' = State__Full)) then
+         trace ↩ Impl__Deq ;;
+         st <=: State__Empty
+    }}.
+
+  Definition shift :=
+    {{ a' <- $a ;;
+       when decide (a' <> 0%bv) then
+         a <=: (a' ≫ 1)%bv
+    }}.
+
+  Definition tick :=
+    {{ st' <- $st ;;
+       when (decide (st' = State__Busy)) then
+         trace ↩ Impl__Tick ;;
+         a' <- $a ;;
+         if (decide (a' = 0%bv)) then
+           st <=: State__Full
+         else
+           shift
+    }}.
+
+  Definition specResult m :=
+    match m with
+    | Spec__Enq _ => unit
+    | Spec__Deq => unit
+    | Spec__Tick => unit
     end.
 
-  Fixpoint predict' st xs :=
-    match xs with
-    | [] => []
-    | x :: xs' => predict_next st x :: predict' (predictor_step st x) xs'
+  Definition runSpec m : ActionValue (specResult m) :=
+    match m with
+    | Spec__Enq a => enq a
+    | Spec__Deq => deq
+    | Spec__Tick => tick
     end.
 
-  Definition predict xs := predict' None xs.
+  Definition runSpec1 m := runAction1 (runSpec m).
+  Definition runSpecs xs := fold_left (fun a b => runSpec1 b a) xs.
 
-  Definition rep (x : State) (y : PredictorState) : Prop :=
-    (exists v, y = Some v /\
-            bv_unsigned x.(R).(r_cnt) = (Z.of_nat v) /\
-            (v <= 3)%nat /\
-            x.(R).(r_busy) = 1
-    )
-    \/ (y = None /\ x.(R).(r_busy) = 0).
+  Definition circuit : Circuit t spec := {| init := mk; run := runSpec1 |}.
+End Spec.
 
-  Lemma simulation_step : forall s1 s2 s1' s2' x,
-      rep s1 s2 ->
-      s1' = circuit_step s1 x ->
-      s2' = predictor_step s2 (public1 x) ->
-      rep s1' s2'.
-  Proof.
-    unfold rep, circuit_step, predictor_step, public1.
-    simplify. inv H.
-    - inv H0 as [v]. inv H. inv H1. inv H0. destruct v as [| v'].
-      + assert (s1.(R).(r_cnt) = 0) by bv_solve.
-        right. rewrite H0. rewrite H2. equality.
-      + left. exists v'. intuition; try lia.
-        * rewrite H2. simplify. pose proof H.
-          apply bv_not_zero_nat_succ in H.
-          rewrite <- bv_eqb_eq in H.
-          apply not_true_is_false in H.
-          replace 0 with (bv_0 2) by bv_solve.
-          rewrite H. simplify. bv_simplify.
-          rewrite H0. unfold bv_wrap, bv_modulus.
-          lia.
-        * rewrite H2. simplify. pose proof H.
-          apply bv_not_zero_nat_succ in H.
-          rewrite <- bv_eqb_eq in H.
-          apply not_true_is_false in H.
-          replace 0 with (bv_0 2) by bv_solve.
-          rewrite H. simplify. equality.
-    - inv H0. rewrite H1. simplify. repeat case_match; try equality.
-      left. exists 3%nat. intuition.
-  Qed.
+Definition invariant s1 s2 :=
+  s1.(Impl.st) = s2.(Spec.st) /\
+    s1.(Impl.a) = s2.(Spec.a) /\
+    s1.(Impl.trace) = s2.(Spec.trace).
 
-  Lemma simulation_initial : rep State0 None.
-  Proof.
-    unfold rep. simplify. right. equality.
-  Qed.
+Ltac t0 :=
+  match goal with
+  | t : Spec.t_inner |- _ => destruct t
+  | t : Impl.t_inner |- _ => destruct t
+  | m : method |- _ => destruct m
+  | s : spec |- _ => destruct s
+  | st : state |- _ => destruct st
+  | |- context [ decide _ ] => case_decide
+  | H : _ /\ _ |- _ => destruct_and! H
+  | |- _ /\ _ => split
+  end.
 
-  Lemma simulation_many_step : forall xs s1 s2 s1' s2',
-    rep s1 s2 ->
-    s1' = circuit_steps s1 xs ->
-    s2' = predictor_steps s2 (public xs) ->
-    rep s1' s2'.
-  Proof.
-    induction xs as [| y ys IHy ]; simplify; try equality.
-    - assert (rep (circuit_step s1 y) (predictor_step s2 (public1 y))).
-      { apply simulation_step with (s1 := s1) (s2 := s2) (x := y); eauto. }
-      unfold circuit_steps, predictor_steps. eapply IHy; eauto.
-  Qed.
+Ltac t1 :=
+  unfold refines, bind, fmap, modify,
+    get, runAction1, runAction,
+    Impl.enq, Spec.enq, Impl.deq, Spec.deq,
+    Impl.tick, Spec.tick, Impl.shift_and_add, Spec.shift,
+    Impl.runMethod1, Spec.runSpec1, Impl.runMethod, Spec.runSpec,
+    Impl.runMethods, Spec.runSpecs, runAction in *.
 
-  Definition leak_next (s : State) (x : I) :=
-    let ready :=
-      if s.(R).(r_busy) =? 1
-      then
-        if s.(R).(r_cnt) =? 0
-        then 1
-        else 0
-      else 0
-    in
-    {| leak_valid := x.(in_valid); leak_ready := ready |}.
+Ltac t2 := t1; simplify; t1; repeat (t0; simplify).
+Ltac t := t2; try (equality || eauto 7).
 
-  Lemma simulation_predict_leak : forall s1 s2 x,
-      rep s1 s2 ->
-      leak_next s1 x = predict_next s2 (public1 x).
-  Proof.
-    unfold leak_next, predict_next, public1, rep.
-    simplify. inv H.
-    - inv H0. inv H. inv H1. inv H0. destruct x0 as [| z].
-      + assert (s1.(R).(r_cnt) = 0) by bv_solve.
-        destruct s1. destruct R0. simplify.
-        assert (in_valid x = 0 \/ in_valid x = 1).
-        { apply bv_1_ind with (P := (fun x => x = 0 \/ x = 1)); eauto. }
-        inv H0.
-        * rewrite H2; simplify. equality.
-        * rewrite H2; simplify. equality.
-      + apply bv_not_zero_nat_succ in H. destruct s1.
-        destruct R0. simplify. rewrite <- bv_eqb_neq in H.
-        replace 0 with (bv_0 2) by bv_solve. rewrite H.
-        assert (in_valid x = 0 \/ in_valid x = 1).
-        { apply bv_1_ind with (P := (fun x => x = 0 \/ x = 1)); eauto. }
-        inv H0.
-        * rewrite H2; simplify. equality.
-        * rewrite H2; simplify. equality.
-    - inv H0. assert (in_valid x = 0 \/ in_valid x = 1).
-      { apply bv_1_ind with (P := (fun x => x = 0 \/ x = 1)); eauto. }
-      inv H.
-      + rewrite H0. simplify. destruct s1. destruct R0. simplify.
-        equality.
-      + rewrite H0. simplify. destruct s1. destruct R0. simplify.
-        equality.
-  Qed.
+Lemma enq_ok : forall s1 s2 a b,
+    invariant s1 s2 ->
+    invariant (runAction1 (Impl.enq a b) s1)
+      (runAction1 (Spec.enq a) s2).
+Proof.
+  unfold invariant in *; t.
+Qed.
 
-  Lemma predict_app' : forall xs ys1 ys2 x s,
-      ys1 = predict' s xs ->
-      ys2 = predict' s (xs ++ [x]) ->
-      ys2 = ys1 ++ [predict_next (predictor_steps s xs) x].
-  Proof.
-    induction xs as [| z zs IHz ]; simplify.
-    - equality.
-    - f_equal. apply IHz; equality.
-  Qed.
+Lemma deq_ok : forall s1 s2,
+    invariant s1 s2 ->
+    invariant (runAction1 Impl.deq s1)
+      (runAction1 Spec.deq s2).
+Proof.
+  unfold invariant in *; t.
+Qed.
 
-  Lemma predict_app : forall xs x,
-      predict (xs ++ [x]) =
-        predict xs ++ [predict_next (predictor_steps None xs) x].
-  Proof.
-    simplify. apply predict_app'; equality.
-  Qed.
+Lemma tick_ok : forall s1 s2,
+    invariant s1 s2 ->
+    invariant (runAction1 Impl.tick s1)
+      (runAction1 Spec.tick s2).
+Proof.
+  unfold invariant in *; t.
+Qed.
 
-  Lemma circuit_steps_app' : forall xs x s1 s2 s3,
-      s2 = circuit_steps s1 xs ->
-      s3 = circuit_steps s1 (xs ++ [x]) ->
-      s3.(T) = s2.(T) ++ [leak_next s2 x].
-  Proof.
-    induction xs as [| z zs IHz ]; simplify.
-    - unfold circuit_step, leak_next.
-      destruct s1 as [R T Y]. destruct R as [a b count busy].
-      simplify. repeat case_match; simplify!; eauto.
-      all: try rewrite H0; eauto.
-    - apply IHz with (s1 := (circuit_step s1 z)); equality.
-  Qed.
+Local Hint Resolve enq_ok deq_ok tick_ok : core.
 
+Theorem refines_ok : refines Impl.circuit Spec.circuit policy invariant.
+Proof.
+  t.
+Qed.
 
-  Lemma circuit_steps_app : forall xs x,
-      T (circuit_steps State0 (xs ++ [x])) =
-        T (circuit_steps State0 xs) ++ [leak_next (circuit_steps State0 xs) x].
-  Proof.
-    simplify. apply circuit_steps_app' with (xs := xs) (s1 := State0); equality.
-  Qed.
+Local Hint Resolve refines_ok : core.
 
-  Theorem circuit_ct : exists f, forall xs s,
-      s = circuit_steps State0 xs -> s.(T) = f (public xs).
-  Proof.
-    exists predict.
-    induction xs as [| z zs IHz ] using rev_ind; simplify.
-    - equality.
-    - rewrite circuit_steps_app. unfold public. rewrite map_app.
-      simplify. rewrite predict_app. rewrite IHz by equality.
-      unfold public. repeat f_equal. apply simulation_predict_leak.
-      apply simulation_many_step with (xs := zs) (s1 := State0) (s2 := None).
-      + apply simulation_initial.
-      + equality.
-      + equality.
-  Qed.
-End ct.
+Lemma invariant_start : invariant Impl.mk Spec.mk.
+Proof.
+  unfold invariant in *; t.
+Qed.
+
+Local Hint Resolve invariant_start : core.
+
+Corollary simulates_ok : policy ⊢ Impl.circuit ⊑ Spec.circuit.
+Proof.
+  unfold simulates in *; exists invariant; t.
+Qed.
+
+Local Hint Resolve simulates_ok : core.
+
+Lemma runMethods_invariant : forall xs,
+    invariant (Impl.runMethods xs Impl.mk)
+      (Spec.runSpecs (map policy xs) Spec.mk).
+Proof.
+  induction xs using rev_ind.
+  - t.
+  - t1. rewrite map_app. repeat rewrite fold_left_app. eauto.
+Qed.
+
+Local Hint Resolve runMethods_invariant : core.
+
+Theorem ct : exists f, forall xs s,
+    s = Impl.runMethods xs Impl.mk ->
+    s.(Impl.trace) = f (map policy xs).
+Proof.
+  exists (fun xs => (Spec.runSpecs xs Spec.mk).(Spec.trace)); intros;
+  pose proof (runMethods_invariant xs); unfold invariant in *; t.
+Qed.
