src/base.v
@@ -9,12 +9,20 @@
 (*                                                                                *)
 (**********************************************************************************)
 
-From stdpp Require Export base tactics list options.
+From stdpp Require Export base tactics list vector options.
 From RecordUpdate Require Export RecordUpdate.
 
 #[export] Set Printing Projections.
 #[export] Set Implicit Arguments.
+#[export] Set Warnings "-notation-for-abbreviation".
 
 Ltac simplify := repeat progress (intros; simpl in *; list_simplifier; subst).
 Ltac equality := intuition congruence.
 Ltac propositional := intuition.
+
+Notation Maybe := @option.
+Definition Valid {t} := Some (A := t).
+Definition Invalid {t} := None (A := t).
+
+Definition Bool := bool.
+Definition Vector n t := Vector.t t n.
