src/circuit.v
@@ -1,4 +1,0 @@
-From research Require Import base bitvector.
-
-Declare Scope circuit_scope.
-Delimit Scope circuit_scope with circuit.
