src/multiplier1.v
@@ -1,0 +1,502 @@
+(**********************************************************************************)
+(*                                                                                *)
+(*             multiplier.v - Shift-and-add 4-bit multiplier.                     *)
+(*                                                                                *)
+(*                   +---------------------------+                                *)
+(*                   |                           |                                *)
+(*           A -----------                 ------|------ P                        *)
+(*                   |                           |                                *)
+(*           B -----------        A*B            |                                *)
+(*                   |                           |                                *)
+(*           V -----------                 ------------- R                        *)
+(*                   |                           |                                *)
+(*                   +---------------------------+                                *)
+(*                                                                                *)
+(*  The main theorem is a statement of a cryptographic constant-time (CCT)        *)
+(*  hyperproperty. The statement of the property looks as follows (which we       *)
+(*  state as an equivalent single-copy trace property):                           *)
+(*                                                                                *)
+(*  There exists some predictor [f] such that given a circuit_step schedule [C],  *)
+(*  starting from a reset state, the multiplier circuit [M] will produce an       *)
+(*  implementation leakage trace [t'].                                            *)
+(*                                                                                *)
+(*  A specification leakage trace [t] is extracted from schedule [C] which        *)
+(*  will record the values of [A] and [valid] each circuit_step. On termination,  *)
+(*                                                                                *)
+(*                              [t' = f t].                                       *)
+(*                                                                                *)
+(**********************************************************************************)
+
+From research Require Import base bitvector.
+
+Local Open Scope bv_scope.
+
+Section definitions.
+  Record Registers :=
+    { r_A : bv 8
+    ; r_B : bv 4
+    ; r_cnt : bv 2
+    ; r_busy : bv 1
+    }.
+
+  Record I :=
+    { in_A : bv 4
+    ; in_B : bv 4
+    ; in_valid : bv 1
+    }.
+
+  Record O :=
+    { out_P : bv 8
+    ; out_ready : bv 1
+    }.
+
+  Definition O0 := {| out_P := 0; out_ready := 0 |}.
+
+  Record ILeakage :=
+    { leak_valid : bv 1
+    ; leak_ready : bv 1
+    }.
+
+  Record State :=
+    { R : Registers
+    ; T : list ILeakage
+    ; Y : list O
+    }.
+
+  Definition State0 :=
+    {| R := {| r_A := 0; r_B := 0; r_cnt := 0; r_busy := 0 |}
+    ; T := []
+    ; Y := [] |}.
+
+  Definition shift_and_add (b : bv 4) (a : bv 8) : bv 8 :=
+    let t0 := bv_extract 4 5 a in
+    let t1 := if a? then 5#b else 0 in
+    t0 + t1 || bv_extract 1 3 a.
+
+  Definition circuit_step (s : State) (x : I) : State :=
+    if s.(R).(r_busy) =? 0
+    then
+      if x.(in_valid) =? 1
+      then
+        let ra' := 8#x.(in_A) in
+        let rb' := x.(in_B) in
+        let rcount' := 3 in
+        let rbusy' := 1 in
+        let r' := {| r_A := ra'; r_B := rb'; r_cnt := rcount'; r_busy := rbusy' |} in
+        let t' := s.(T) ++ [{| leak_valid := 1; leak_ready := 0 |}] in
+        let y' := s.(Y) ++ [O0] in
+        {| R := r'; T := t'; Y := y' |}
+      else
+        let t' := s.(T) ++ [{| leak_valid := 0; leak_ready := 0 |}] in
+        let r' := s.(R) in
+        let y' := s.(Y) ++ [O0] in
+        {| R := r'; T := t'; Y := y' |}
+    else
+      let ra' := shift_and_add s.(R).(r_B) s.(R).(r_A) in
+      let rb' := s.(R).(r_B) in
+      if s.(R).(r_cnt) =? 0
+      then
+        let rcount' := 0 in
+        let rbusy' := 0 in
+        let r' := {| r_A := ra'; r_B := rb'; r_cnt := rcount'; r_busy := rbusy' |} in
+        let t' := s.(T) ++ [{| leak_valid := x.(in_valid); leak_ready := 1 |}] in
+        let y' := s.(Y) ++ [{| out_P := ra'; out_ready := 1 |}] in
+        {| R := r'; T := t'; Y := y' |}
+      else
+        let rcount' := bv_pred s.(R).(r_cnt) in
+        let rbusy' := 1 in
+        let r' := {| r_A := ra'; r_B := rb'; r_cnt := rcount'; r_busy := rbusy' |} in
+        let t' := s.(T) ++ [{| leak_valid := x.(in_valid); leak_ready := 0 |}] in
+        let y' := s.(Y) ++ [O0] in
+        {| R := r'; T := t'; Y := y' |}.
+
+  Definition circuit_steps s xs := fold_left circuit_step xs s.
+End definitions.
+
+Section correctness.
+  Fixpoint repeat {A : Type} (f : A -> A) (n : nat) {struct n} : (A -> A) :=
+    match n with
+    | 0%nat => id
+    | S n' => f ∘ repeat f n'
+    end.
+
+  Definition repeat_shift_and_add n b a := (repeat (shift_and_add b) n) a.
+
+  Definition shift_and_add4 := repeat_shift_and_add 4.
+
+  Definition shift_and_add' (b a : Z) :=
+    Z.lor (bv_wrap 5 (a ≫ 4 + (bv_wrap 1 a * b)) ≪ 3) (bv_wrap 3 (a ≫ 1)).
+
+  Definition repeat_shift_and_add' n b a := (repeat (shift_and_add' b) n) a.
+
+  Definition shift_and_add4' := repeat_shift_and_add' 4.
+
+  Lemma shift_and_add_equiv : forall a b,
+      shift_and_add' (bv_unsigned b) (bv_unsigned a) =
+        bv_unsigned (shift_and_add b a).
+  Proof.
+    intros a b. unfold shift_and_add, shift_and_add'. bv_simplify.
+    unfold Z.of_N, bv_odd.
+    unfold bv_wrap. rewrite Zmod_odd. case_match.
+    - replace (1 * bv_unsigned b)%Z with (bv_unsigned b) by lia. bv_solve.
+    - Search (0 * _)%Z. rewrite Z.mul_0_l. bv_solve.
+  Qed.
+
+  Lemma shift_and_add_repeat_equiv : forall n a b,
+      (repeat_shift_and_add' n) (bv_unsigned b) (bv_unsigned a) =
+        bv_unsigned (repeat_shift_and_add n b a).
+  Proof.
+    intros n a b. induction n; simplify.
+    - unfold repeat_shift_and_add', repeat_shift_and_add. equality.
+    - unfold repeat_shift_and_add', repeat_shift_and_add in *. simplify.
+      rewrite IHn. apply shift_and_add_equiv.
+  Qed.
+
+  Lemma shift_and_add4_equiv : forall a b,
+      shift_and_add4' (bv_unsigned b) (bv_unsigned a) =
+        bv_unsigned (shift_and_add4 b a).
+  Proof.
+    unfold shift_and_add4', shift_and_add4. apply shift_and_add_repeat_equiv.
+  Qed.
+
+  (* Tactic for exhaustive case analysis on integers in range [0,16) *)
+  (* Automatically finds variables with range hypotheses and does case analysis *)
+  Ltac by_cases16 :=
+    repeat match goal with
+      | [ H : (0 <= ?z < 16)%Z |- _ ] =>
+          let Hz := fresh "Hcases" in
+          assert (z = 0 \/ z = 1 \/ z = 2 \/ z = 3 \/ z = 4 \/ z = 5 \/ z = 6 \/ z = 7 \/
+                    z = 8 \/ z = 9 \/ z = 10 \/ z = 11 \/ z = 12 \/ z = 13 \/ z = 14 \/ z = 15)%Z
+            as Hz by lia; clear H;
+          destruct_or?; subst
+      end; equality.
+
+  Lemma shift_and_add4'_multiplies : forall a b,
+      (0 <= a < bv_modulus 4%N)%Z ->
+      (0 <= b < bv_modulus 4%N)%Z ->
+      shift_and_add4' b a = (a * b)%Z.
+  Proof.
+    intros a b Ha Hb.
+    replace (bv_modulus 4%N) with 16%Z in * by reflexivity.
+    by_cases16.
+  Qed.
+
+  Lemma shift_and_add4_multiplies : forall (a b : bv 4),
+      bv_unsigned (shift_and_add4 b (8#a)) = (bv_unsigned a * bv_unsigned b)%Z.
+  Proof.
+    intros a b. rewrite <- shift_and_add4_equiv.
+    Search bv_unsigned bv_zero_extend. rewrite bv_zero_extend_unsigned by lia.
+    apply shift_and_add4'_multiplies. all: bv_solve.
+  Qed.
+
+  Notation "a *| b" := ((8#a) * (8#b)) (at level 35).
+
+  Lemma shift_and_add4_correct : forall (a b : bv 4),
+      shift_and_add4 b (8#a) = a *| b.
+  Proof.
+    intros a b. Search (bv_unsigned _ = bv_unsigned _).
+    rewrite bv_eq. Search bv_mul.
+    rewrite bv_mul_unsigned.
+    Search bv_zero_extend bv_unsigned.
+    repeat rewrite bv_zero_extend_unsigned by lia.
+    Check bv_wrap_small. rewrite bv_wrap_small.
+    - apply shift_and_add4_multiplies.
+    - bv_saturate_unsigned. unfold bv_modulus in *; simplify. nia.
+  Qed.
+
+  Definition busy (s : State) := s.(R).(r_busy) = 1.
+  Definition finished (s : State) := s.(R).(r_cnt) = 0.
+  Definition valid (x : I) := x.(in_valid) = 1.
+
+  Definition circuit_step_idle_valid s1 x s2 : Prop :=
+    ~ busy s1 -> valid x -> s2 = circuit_step s1 x ->
+    s2 = s1 <| R := {| r_A := 8#x.(in_A); r_B := x.(in_B); r_cnt := 3; r_busy := 1 |} |>
+            <| T := s1.(T) ++ [{| leak_valid := 1; leak_ready := 0 |}] |>
+            <| Y := s1.(Y) ++ [O0] |>.
+
+  Lemma circuit_step_idle_valid_holds : forall s1 x s2, circuit_step_idle_valid s1 x s2.
+  Proof.
+    unfold circuit_step_idle_valid. simplify.
+    unfold circuit_step in *. unfold busy in *.
+    unfold valid in *. rewrite <- bv_eqb_neq in H.
+    simplify!. rewrite H0. rewrite H.
+    simplify. equality.
+  Qed.
+
+  Definition circuit_step_idle_invalid s1 x s2 : Prop :=
+    ~ busy s1 -> ~ valid x -> s2 = circuit_step s1 x ->
+    s2 = s1 <| T := s1.(T) ++ [{| leak_valid := 0; leak_ready := 0 |}] |>
+            <| Y := s1.(Y) ++ [O0] |>.
+
+  Lemma circuit_step_idle_invalid_holds : forall s1 x s2, circuit_step_idle_invalid s1 x s2.
+  Proof.
+    unfold circuit_step_idle_invalid. simplify.
+    unfold circuit_step, busy, valid in *.
+    simplify!. rewrite H. rewrite H0.
+    simplify. equality.
+  Qed.
+
+  Definition circuit_step_busy_unfinished s1 x s2 : Prop :=
+    busy s1 -> ~ finished s1 -> s2 = circuit_step s1 x ->
+    s2 = s1 <| R; r_A := shift_and_add s1.(R).(r_B) s1.(R).(r_A) |>
+            <| R; r_cnt := bv_pred s1.(R).(r_cnt)|>
+            <| T := s1.(T) ++ [{| leak_valid := x.(in_valid); leak_ready := 0 |}] |>
+            <| Y := s1.(Y) ++ [O0] |> .
+
+  Lemma circuit_step_busy_unfinished_holds : forall s1 x s2, circuit_step_busy_unfinished s1 x s2.
+  Proof.
+    unfold circuit_step_busy_unfinished. simplify.
+    unfold circuit_step, busy, finished in *.
+    simplify!. rewrite H.
+    simplify. rewrite <- bv_eqb_neq in H0. rewrite H0.
+    equality.
+  Qed.
+
+  Definition circuit_step_busy_finished s1 x s2 : Prop :=
+    busy s1 -> finished s1 -> s2 = circuit_step s1 x ->
+    s2 = s1 <| R; r_A := shift_and_add s1.(R).(r_B) s1.(R).(r_A) |>
+            <| R; r_cnt := 0 |>
+            <| R; r_busy := 0 |>
+            <| T := s1.(T) ++ [{| leak_valid := x.(in_valid); leak_ready := 1 |}] |>
+            <| Y := s1.(Y) ++ [{|
+                             out_P := shift_and_add s1.(R).(r_B) s1.(R).(r_A);
+                             out_ready := 1
+                           |}]
+              |>.
+
+  Lemma circuit_step_busy_finished_holds : forall s1 x s2, circuit_step_busy_finished s1 x s2.
+  Proof.
+    unfold circuit_step_busy_finished. simplify.
+    unfold circuit_step, busy, finished in *.
+    rewrite H0. simplify!. rewrite H.
+    simplify. equality.
+  Qed.
+
+  Tactic Notation "unfold*" :=
+    unfold circuit_step_idle_valid, circuit_step_idle_invalid, circuit_step_busy_unfinished,
+      circuit_step_busy_finished, circuit_steps, busy, finished, shift_and_add4,
+      valid, repeat_shift_and_add, repeat, compose in *.
+
+  (* Finally, with all those helper theorems out of the way, we can now prove
+     the following correctness property:
+
+     For any circuit_step where the circuit is idle, if a valid [a] and [b] are
+     provided, four circuit_steps later it will produce [a *| b]. *)
+
+  Theorem circuit_steps_correct: forall s1 x1 s2 x2 s3 x3 s4 x4 s5 x5 s6 a b,
+      ~ busy s1 ->
+      x1 = {| in_A := a; in_B := b; in_valid := 1 |} ->
+      s2 = circuit_step s1 x1 ->
+      s3 = circuit_step s2 x2 ->
+      s4 = circuit_step s3 x3 ->
+      s5 = circuit_step s4 x4 ->
+      s6 = circuit_step s5 x5 ->
+      s6.(Y) = s1.(Y) ++ [O0; O0; O0; O0; {| out_P := a *| b; out_ready := 1 |}].
+  Proof.
+    intros. rewrite <- shift_and_add4_correct. unfold*. simpl in *.
+
+    1: apply circuit_step_idle_valid_holds      in H1.
+    1: apply circuit_step_busy_unfinished_holds in H2.
+    1: apply circuit_step_busy_unfinished_holds in H3.
+    1: apply circuit_step_busy_unfinished_holds in H4.
+    1: apply circuit_step_busy_finished_holds   in H5.
+
+    all: unfold*; simplify; solve [ eauto | bv_solve ].
+  Qed.
+End correctness.
+
+Section ct.
+  Definition SLeakage := option unit.
+
+  Definition public1 x := if x.(in_valid) =? 1 then Some tt else None.
+
+  Definition public := map public1.
+
+  Definition PredictorState := option nat.
+
+  Definition predictor_step (st : PredictorState) (s : SLeakage) :=
+    match st with
+    | Some (S n) => Some n
+    | Some 0%nat => None
+    | None =>
+        match s with
+        | Some _ => Some 3%nat
+        | None   => None
+        end
+    end.
+
+  Definition predictor_steps (st : PredictorState) (xs : list SLeakage) :=
+    fold_left predictor_step xs st.
+
+  Definition predict_next (st : PredictorState) (s : SLeakage) :=
+    match st with
+    | Some 0%nat =>
+        match s with
+        | Some _ => {| leak_valid := 1; leak_ready := 1 |}
+        | None => {| leak_valid := 0; leak_ready := 1 |}
+        end
+    | _ =>
+        match s with
+        | Some _ => {| leak_valid := 1; leak_ready := 0 |}
+        | None => {| leak_valid := 0; leak_ready := 0 |}
+        end
+    end.
+
+  Fixpoint predict' st xs :=
+    match xs with
+    | [] => []
+    | x :: xs' => predict_next st x :: predict' (predictor_step st x) xs'
+    end.
+
+  Definition predict xs := predict' None xs.
+
+  Definition rep (x : State) (y : PredictorState) : Prop :=
+    (exists v, y = Some v /\
+            bv_unsigned x.(R).(r_cnt) = (Z.of_nat v) /\
+            (v <= 3)%nat /\
+            x.(R).(r_busy) = 1
+    )
+    \/ (y = None /\ x.(R).(r_busy) = 0).
+
+  Lemma simulation_step : forall s1 s2 s1' s2' x,
+      rep s1 s2 ->
+      s1' = circuit_step s1 x ->
+      s2' = predictor_step s2 (public1 x) ->
+      rep s1' s2'.
+  Proof.
+    unfold rep, circuit_step, predictor_step, public1.
+    simplify. inv H.
+    - inv H0 as [v]. inv H. inv H1. inv H0. destruct v as [| v'].
+      + assert (s1.(R).(r_cnt) = 0) by bv_solve.
+        right. rewrite H0. rewrite H2. equality.
+      + left. exists v'. intuition; try lia.
+        * rewrite H2. simplify. pose proof H.
+          apply bv_not_zero_nat_succ in H.
+          rewrite <- bv_eqb_eq in H.
+          apply not_true_is_false in H.
+          replace 0 with (bv_0 2) by bv_solve.
+          rewrite H. simplify. bv_simplify.
+          rewrite H0. unfold bv_wrap, bv_modulus.
+          lia.
+        * rewrite H2. simplify. pose proof H.
+          apply bv_not_zero_nat_succ in H.
+          rewrite <- bv_eqb_eq in H.
+          apply not_true_is_false in H.
+          replace 0 with (bv_0 2) by bv_solve.
+          rewrite H. simplify. equality.
+    - inv H0. rewrite H1. simplify. repeat case_match; try equality.
+      left. exists 3%nat. intuition.
+  Qed.
+
+  Lemma simulation_initial : rep State0 None.
+  Proof.
+    unfold rep. simplify. right. equality.
+  Qed.
+
+  Lemma simulation_many_step : forall xs s1 s2 s1' s2',
+    rep s1 s2 ->
+    s1' = circuit_steps s1 xs ->
+    s2' = predictor_steps s2 (public xs) ->
+    rep s1' s2'.
+  Proof.
+    induction xs as [| y ys IHy ]; simplify; try equality.
+    - assert (rep (circuit_step s1 y) (predictor_step s2 (public1 y))).
+      { apply simulation_step with (s1 := s1) (s2 := s2) (x := y); eauto. }
+      unfold circuit_steps, predictor_steps. eapply IHy; eauto.
+  Qed.
+
+  Definition leak_next (s : State) (x : I) :=
+    let ready :=
+      if s.(R).(r_busy) =? 1
+      then
+        if s.(R).(r_cnt) =? 0
+        then 1
+        else 0
+      else 0
+    in
+    {| leak_valid := x.(in_valid); leak_ready := ready |}.
+
+  Lemma simulation_predict_leak : forall s1 s2 x,
+      rep s1 s2 ->
+      leak_next s1 x = predict_next s2 (public1 x).
+  Proof.
+    unfold leak_next, predict_next, public1, rep.
+    simplify. inv H.
+    - inv H0. inv H. inv H1. inv H0. destruct x0 as [| z].
+      + assert (s1.(R).(r_cnt) = 0) by bv_solve.
+        destruct s1. destruct R0. simplify.
+        assert (in_valid x = 0 \/ in_valid x = 1).
+        { apply bv_1_ind with (P := (fun x => x = 0 \/ x = 1)); eauto. }
+        inv H0.
+        * rewrite H2; simplify. equality.
+        * rewrite H2; simplify. equality.
+      + apply bv_not_zero_nat_succ in H. destruct s1.
+        destruct R0. simplify. rewrite <- bv_eqb_neq in H.
+        replace 0 with (bv_0 2) by bv_solve. rewrite H.
+        assert (in_valid x = 0 \/ in_valid x = 1).
+        { apply bv_1_ind with (P := (fun x => x = 0 \/ x = 1)); eauto. }
+        inv H0.
+        * rewrite H2; simplify. equality.
+        * rewrite H2; simplify. equality.
+    - inv H0. assert (in_valid x = 0 \/ in_valid x = 1).
+      { apply bv_1_ind with (P := (fun x => x = 0 \/ x = 1)); eauto. }
+      inv H.
+      + rewrite H0. simplify. destruct s1. destruct R0. simplify.
+        equality.
+      + rewrite H0. simplify. destruct s1. destruct R0. simplify.
+        equality.
+  Qed.
+
+  Lemma predict_app' : forall xs ys1 ys2 x s,
+      ys1 = predict' s xs ->
+      ys2 = predict' s (xs ++ [x]) ->
+      ys2 = ys1 ++ [predict_next (predictor_steps s xs) x].
+  Proof.
+    induction xs as [| z zs IHz ]; simplify.
+    - equality.
+    - f_equal. apply IHz; equality.
+  Qed.
+
+  Lemma predict_app : forall xs x,
+      predict (xs ++ [x]) =
+        predict xs ++ [predict_next (predictor_steps None xs) x].
+  Proof.
+    simplify. apply predict_app'; equality.
+  Qed.
+
+  Lemma circuit_steps_app' : forall xs x s1 s2 s3,
+      s2 = circuit_steps s1 xs ->
+      s3 = circuit_steps s1 (xs ++ [x]) ->
+      s3.(T) = s2.(T) ++ [leak_next s2 x].
+  Proof.
+    induction xs as [| z zs IHz ]; simplify.
+    - unfold circuit_step, leak_next.
+      destruct s1 as [R T Y]. destruct R as [a b count busy].
+      simplify. repeat case_match; simplify!; eauto.
+      all: try rewrite H0; eauto.
+    - apply IHz with (s1 := (circuit_step s1 z)); equality.
+  Qed.
+
+
+  Lemma circuit_steps_app : forall xs x,
+      T (circuit_steps State0 (xs ++ [x])) =
+        T (circuit_steps State0 xs) ++ [leak_next (circuit_steps State0 xs) x].
+  Proof.
+    simplify. apply circuit_steps_app' with (xs := xs) (s1 := State0); equality.
+  Qed.
+
+  Theorem circuit_ct : exists f, forall xs s,
+      s = circuit_steps State0 xs -> s.(T) = f (public xs).
+  Proof.
+    exists predict.
+    induction xs as [| z zs IHz ] using rev_ind; simplify.
+    - equality.
+    - rewrite circuit_steps_app. unfold public. rewrite map_app.
+      simplify. rewrite predict_app. rewrite IHz by equality.
+      unfold public. repeat f_equal. apply simulation_predict_leak.
+      apply simulation_many_step with (xs := zs) (s1 := State0) (s2 := None).
+      + apply simulation_initial.
+      + equality.
+      + equality.
+  Qed.
+End ct.
