src/simulates.v
@@ -1,0 +1,23 @@
+From research Require Import base program.
+
+Record Circuit t m :=
+  { run : m -> t -> t
+  ; init : t
+  }.
+
+Definition refines
+  `(c1 : Circuit t1 m1)
+  `(c2 : Circuit t2 m2)
+  (policy : m1 -> m2)
+  (R : t1 -> t2 -> Prop) :=
+  forall s1 s2,
+    R s1 s2 ->
+    (forall m s1' s2',
+        s1' = c1.(run) m s1 ->
+        s2' = c2.(run) (policy m) s2 ->
+        R s1' s2').
+
+Definition simulates `(c1 : Circuit t1 m1) `(c2 : Circuit t2 m2) (policy : m1 -> m2) :=
+  exists R, R c1.(init) c2.(init) /\ refines c1 c2 policy R.
+
+Notation "P ⊢ c1 ⊑ c2" := (simulates c1 c2 P) (at level 60, c1 at next level).
